src/program_proof/simplepb/pb_init_proof.v
@@ -2,7 +2,8 @@ From Perennial.base_logic Require Import lib.saved_prop.
 From Perennial.program_proof Require Import grove_prelude.
 From Goose.github_com.mit_pdos.gokv.simplepb Require Export pb.
 From Perennial.program_proof.simplepb Require Export pb_protocol.
-From Perennial.program_proof.simplepb Require Import pb_definitions.
+From Perennial.program_proof.simplepb Require Import pb_definitions config_protocol_proof
+     clerk_proof.
 From Perennial.program_proof.grove_shared Require Import urpc_spec.
 From iris.algebra Require Import mono_list.
 
@@ -16,21 +17,6 @@ Notation compute_reply := (Sm.compute_reply pb_record).
 Notation pbG := (pbG (pb_record:=pb_record)).
 Context `{!gooseGlobalGS Σ}.
 Context `{!pbG Σ}.
-
-Lemma alloc_simplepb_server γ γsrv :
-  is_sys_init_witness γ.(s_pb) -∗
-  own_replica_ghost γ.(s_pb) γsrv.(r_pb) (U64 0) [] false -∗
-  own_primary_escrow_ghost γ.(s_prim) γsrv.(r_prim) 0 -∗
-  is_proposal_facts_prim γ.(s_prim) 0 [] -∗
-  is_in_config γ γsrv (U64 0) -∗
-  own_Server_ghost_f γ γsrv (U64 0) [] false.
-Proof.
-  iIntros "#H1 Hpre1 Hpre2 #? #?".
-  (* iDestruct (pb_ghost_server_init with "H1 Hpre") as "[Hrep Hprim]". *)
-  iExists [].
-  iSplitR; first done.
-  iFrame "∗#".
-Qed.
 
 Definition pb_spec_list γ γsrv :=
   [ (U64 0, ApplyAsBackup_spec γ γsrv) ;
@@ -58,29 +44,41 @@ Proof.
   set_solver.
 Qed.
 
+Definition is_pb_sys_init_witness γ γsrv : iProp Σ :=
+  is_sys_init_witness γ.(s_pb) ∗
+  is_in_config γ γsrv (U64 0) ∗
+  is_proposal_facts_prim γ.(s_prim) 0%Z []
+.
+
+Definition is_server_prealloc_witness γsrv : iProp Σ :=
+  is_accepted_lb γsrv.(r_pb) (U64 0) [] ∗ is_epoch_lb γsrv.(r_pb) 0
+.
+
+Lemma prealloc_simplepb_server :
+  ⊢ |={⊤}=> ∃ γsrv,
+  is_server_prealloc_witness γsrv ∗
+  (∀ γ, is_pb_sys_init_witness γ γsrv -∗ own_Server_ghost_f γ γsrv (U64 0) [] false).
+Proof.
+  iMod (pb_ghost_server_pre_init) as (γpb) "(Hpre & #? & #?)".
+  iMod (alloc_primary_protocol_server) as (γprim) "Hprim".
+  iExists {| r_pb := γpb ; r_prim := γprim |}.
+  iModIntro. iFrame "#".
+  iIntros (?) "#(? & ? & ?)".
+  iDestruct (pb_ghost_server_init with "[$] [$]") as "H".
+  by iExists _; iFrame "∗#".
+Qed.
 (* Invariants:
    is_repl_inv
-   is_conf_inv
-   is_helping_inv
    is_preread_inv
+   is_helping_inv
+   is_conf_inv
  *)
 
-(* FIXME: *)
-(*
-Lemma alloc_system :
-  own_ghost γsys [] ={⊤}=∗
-  ∃ γ, own_log γ [] ∗ is_helping_inv γ.(s_log) γsys
-.
-
 Lemma alloc_helping_inv γ :
-  own_ghost γsys [] ={⊤}=∗
-  ∃ γ, own_log γ [] ∗ is_helping_inv γ.(s_log) γsys
-.
+  own_pre_log γ.(s_prelog) [] -∗ own_int_log γ []
+  ={⊤}=∗ is_helping_inv γ.
 Proof.
-  iIntros "Hghost".
-  iMod (own_alloc (●ML [])) as (γ.(s_log)) "[Hlog1 Hlog2]".
-  { apply mono_list_auth_valid. }
-  iExists _; iFrame "Hlog2".
+  iIntros "Hprelog Hint_log".
   iMod (inv_alloc with "[-]") as "$"; last done.
   iNext.
   iExists [].
@@ -101,6 +99,48 @@ Proof.
   apply (f_equal length) in H.
   rewrite app_length /= in H.
   lia.
-Qed. *)
+Qed.
+
+Lemma alloc_simplepb_system γsrvs :
+  length γsrvs > 0 →
+  (∀ γsrv, ⌜γsrv ∈ γsrvs⌝ → is_accepted_lb γsrv.(r_pb) (U64 0) [] ∗ is_epoch_lb γsrv.(r_pb) 0)
+  ={⊤}=∗ ∃ γ,
+  is_pb_system_invs γ ∗
+  own_op_log γ [] ∗
+  (∀ γsrv, ⌜γsrv ∈ γsrvs⌝ → is_pb_sys_init_witness γ γsrv) ∗
+  pb_init_for_config γ.(s_pb) (r_pb <$> γsrvs) ∗
+  primary_init_for_config γ.(s_prim) ∗
+  is_proph_read_inv γ
+.
+Proof.
+  iIntros (?) "#Hpre".
+  iMod alloc_primary_protocol as (γprim) "[Hprim #HprimWit]".
+  iMod (pb_system_init (r_pb <$> γsrvs) with "[]") as (γpb) "Hpb".
+  { by rewrite fmap_length. }
+  { iIntros.
+    apply elem_of_list_fmap_2 in H0 as (? & ? & ?); subst.
+    by iApply "Hpre". }
+  iDestruct "Hpb" as "(#Hrep & Hlog & Hinit & #Hwit)".
+  iMod (alloc_pb_preread_protocol with "Hlog") as (γprelog γreads) "[#Hpreread Hlog]".
+  iMod (own_alloc (●ML [])) as (γintlog) "[Hintlog Hintlog2]".
+  { apply mono_list_auth_valid. }
+  iMod (own_alloc (●ML [])) as (γoplog) "[Hoplog Hoplog2]".
+  { apply mono_list_auth_valid. }
+
+  set (γ:={| s_pb:=γpb ; s_prim:=γprim ; s_prelog := γprelog ; s_internal_log := γintlog ;
+             s_reads:=γreads ; s_log := γoplog
+          |}).
+  iMod (alloc_helping_inv γ with "Hlog Hintlog2") as "#Hhelp".
+  iAssert (|={⊤}=> is_proph_read_inv γ)%I with "[Hintlog Hoplog2]" as ">#Hproph_read_inv".
+  { iApply (inv_alloc with "[Hintlog Hoplog2]").
+    iExists _; iFrame. }
+  iModIntro. iExists γ.
+  iNamed "Hinit".
+  iFrame "∗ His_conf #".
+  iIntros.
+  iExists _; iFrame "#".
+  iPureIntro.
+  by apply elem_of_list_fmap_1.
+Qed.
 
 End pb_init_proof.
